\begin{align}
\frac{2G \nu \omega^2}{m R} ( n^a n^b (-\frac{8}{3} ( Seffp\cdot Seffm) + \frac{2}{3} (\ell\cdot Seffp) (\ell\cdot Seffm) + \frac{40}{3} (n\cdot Seffp) (n\cdot Seffm) ) + \lambda^a \lambda^b ( \frac{2}{3} ( Seffp\cdot Seffm) + \frac{4}{3} (\ell\cdot Seffp) (\ell\cdot Seffm) - \frac{10}{3} (n\cdot Seffp) (n\cdot Seffm) ) -2 n^a \lambda^b ( (n\cdot Seffp) (\lambda\cdot Seffm)+ (n\cdot Seffm) (\lambda\cdot Seffp)) -3 (n\cdot Seffp) n^a \Seffm^b - 3 (n\cdot Seffm) n^a \Seffp^b )
\end{align}
